CompPoly/Fields/BN254/Fast/UInt128L.lean
@@ -1,0 +1,28 @@
+/-
+Copyright (c) 2026 CompPoly Contributors. All rights reserved.
+Released under Apache 2.0 license as described in the file LICENSE.
+Authors: Georgios Raikos
+-/
+
+import CompPoly.Fields.BN254.Fast.Limb
+
+namespace BN254.Fast
+
+structure UInt128L where
+  lo : UInt64
+  hi : UInt64
+deriving DecidableEq
+
+def UInt128L.toNat (x : UInt128L) : Nat :=
+  x.lo.toNat + (x.hi.toNat <<< 64)
+
+
+@[inline] def UInt128L.add (a b : UInt128L) : UInt128L :=
+  let (lo, c0) := addc a.lo b.lo 0
+  let (hi, _) := addc a.hi b.hi c0
+  ⟨ lo, hi ⟩
+
+instance : Add UInt128L := ⟨ UInt128L.add ⟩
+
+
+end BN254.Fast
